\chapter{集合}
\begin{Ex}
设$A$，$B$，$C$是集合，证明$(A\bigtriangleup B)\bigtriangleup C =
A\bigtriangleup (B\bigtriangleup C)$。
\end{Ex}
\begin{proof}[证明]
  
  因为
  \begin{equation}
  x \in A \bigtriangleup B \Leftrightarrow
  (x \in A \land x \notin B) \lor (x \notin A \land x
  \in B),    
  \end{equation}

  所以
  \begin{equation}
    \begin{split}
      x \notin A \bigtriangleup B &\Leftrightarrow
  (x \notin A \lor x \in B) \land (x \in A \lor x
  \notin B)\\
  &\Leftrightarrow (x \notin A \land x \notin B) \lor (x \in A \land x \in B )
    \end{split}
  \end{equation}

  于是
  \begin{equation}\label{xor1}
    \begin{split}
      &x \in (A \bigtriangleup B) \bigtriangleup C\\
      &\Leftrightarrow (x \in A \bigtriangleup B \land x \notin C) \lor (x \notin A \bigtriangleup B \land x \in C)\\
      &\Leftrightarrow (((x \in A \land x \notin B) \lor (x \notin A \land x \in B)) \land x \notin C)\\
      &\lor (((x \notin A \land x \notin B) \lor (x \in A \land x \in B )) \land x \in C)\\
      &\Leftrightarrow (x \in A \land x \notin B \land x \notin C) \lor (x \notin A \land x \in B \land x \notin C)\\
      &\lor (x \notin A \land x \notin B \land x \in C) \lor (x \in A \land x \in B \land x \in C)
    \end{split}
  \end{equation}

  \begin{equation}\label{xor2}
    \begin{split}
      &x \in A \bigtriangleup (B \bigtriangleup C)\\
      &\Leftrightarrow x \in (B \bigtriangleup C) \bigtriangleup A\\
      &\Leftrightarrow (x \in A \land x \notin B \land x \notin C) \lor (x \notin A \land x \in B \land x \notin C)\\
      &\lor (x \notin A \land x \notin B \land x \in C) \lor (x \in A \land x \in B \land x \in C)
    \end{split}
  \end{equation}
  其中\eqref{xor2}式的第二行由对称差运算的交换律得到，\eqref{xor2}式的第三行由与
   \eqref{xor1}式的对称性得到。

  由\eqref{xor1}式和\eqref{xor2}式可得
  $(A\bigtriangleup B)\bigtriangleup C = A\bigtriangleup (B\bigtriangleup C)$。
\end{proof}

\begin{Ex}
设$A$，$B$，$C$，$D$是任意四个集合，证明$(A\cap B) \times (C \cap D) = (A
\times C)
\cap (B \times D)$。
\end{Ex}
\begin{proof}[证明]
  \begin{equation*}
    \begin{split}
    &(x,y) \in (A\cap B) \times (C \cap D)\\
    \Leftrightarrow&x \in A \cap B \text{且} y \in C \cap D\\
    \Leftrightarrow&x \in A \text{且} x \in B \text{且} y \in C \text{且} y \in D\\
    \Leftrightarrow&x \in A \text{且} y \in C \text{且} x \in B \text{且} y \in D\\
    \Leftrightarrow&(x,y) \in A \times C \text{且} (x,y) \in B \times D\\
    \Leftrightarrow&(x,y) \in (A\times C)\cap (B \times D)
    \end{split}
  \end{equation*}
\end{proof}

%%% Local Variables:
%%% mode: latex
%%% TeX-master: "book"
%%% End:
